<!-- 
License: CC BY-SA 4.0 (see LICENSE-CC.md)
-->

# 10. Arithmetic Operations via KMR Transformations

## 10.1 Introduction
This section demonstrates how fundamental arithmetic operations (addition and subtraction) can be expressed through KMR operators, further extending the algebraic framework of KMR transformations. The results show that linear arithmetic emerges as a special case of nonlinear KMR composition, reinforcing the paradigm where nonlinearity represents the fundamental nature of mathematical operations.

## 10.2 Foundational KMR Properties for Arithmetic

### 10.2.1 Basic Operator Definitions
- **Direct KMR operator**: $A ⊙ K = \frac{A}{1 + K \cdot A}$
- **Inverse KMR operator**: $A ⊘ K = \frac{A}{1 - K \cdot A}$

### 10.2.2 Core Algebraic Properties
1. **Inversion Identity**: $(A ⊙ K) ⊘ K = A = (A ⊘ K) ⊙ K$
2. **Group Property**: $(A ⊙ K) ⊙ C = A ⊙ (K + C)$
3. **Non-Commutativity**: $A ⊙ K ≠ K ⊙ A$ and $A ⊘ K ≠ K ⊘ A$
4. **Non-Associativity**: $(A ⊙ K) ⊙ C ≠ A ⊙ (K ⊙ C)$
5. **Scaling Property**: $L \cdot (A ⊙ K) = (L \cdot A) ⊙ (K/L)$
6. **Parameter Extraction**:
   - If $A ⊙ K = X$, then $K = (X ⊘ \frac{1}{A})^{-1}$
   - If $A ⊘ K = X$, then $K = - (X ⊘ \frac{1}{A})^{-1} = [(-X) ⊘ \frac{-1}{A}]^{-1}$

**Proof of Scaling Property**:  
$$[L \cdot (A ⊙ K) = L \cdot \frac{A}{1 + K \cdot A} = \frac{L \cdot A}{1 + K \cdot A}]$$  
$$[(L \cdot A) ⊙ (K/L) = \frac{L \cdot A}{1 + (K/L) \cdot (L \cdot A)} = \frac{L \cdot A}{1 + K \cdot A}]$$  
Thus, $L \cdot (A ⊙ K) = (L \cdot A) ⊙ (K/L) \square$

**Proof of Revised Parameter Extraction**:
From the definition, if $A ⊘ K = X$, then:  
$$[X = \frac{A}{1 - K \cdot A} \implies X(1 - K \cdot A) = A \implies X - X \cdot K \cdot A = A]$$  
$$[- X \cdot K \cdot A = A - X \implies K = \frac{X - A}{A \cdot X} = \frac{1}{A} - \frac{1}{X}]$$

Now verify both forms:  
$$1.[X ⊘ \frac{1}{A} = \frac{X}{1 - \frac{1}{A} \cdot X} = \frac{X}{1 - \frac{X}{A}} = \frac{X}{\frac{A - X}{A}} = \frac{A \cdot X}{A - X}]$$  
$$[(X ⊘ \frac{1}{A})^{-1} = \frac{A - X}{A \cdot X} \implies - (X ⊘ \frac{1}{A})^{-1} = \frac{X - A}{A \cdot X} = K]$$  
$$2.[(-X) ⊘ \frac{-1}{A} = \frac{-X}{1 - (-\frac{1}{A}) \cdot (-X)} = \frac{-X}{1 - \frac{X}{A}} = \frac{-X}{\frac{A - X}{A}} = \frac{-A \cdot X}{A - X}]$$  
$$[(-X) ⊘ \frac{-1}{A}]^{-1} = \frac{A - X}{-A \cdot X} = \frac{X - A}{A \cdot X} = K]$$

Both forms are equivalent and correct.

## 10.3 Addition Through KMR Operators

### 10.3.1 General Case Expression
For any $A ≠ 0$, the sum of two parameters $K$ and $C$ can be expressed as:  
$$K + C = \left( \left( (A ⊙ K) ⊙ C \right) ⊘ \frac{1}{A} \right)^{-1}$$

### 10.3.2 Special Case (A = 1)
When $A = 1$, the expression simplifies to:  
$$K + C = \left( \left( (1 ⊙ K) ⊙ C \right) ⊘ 1 \right)^{-1}$$

### 10.3.3 Proof
Let $Y = (A ⊙ K) ⊙ C$. From the group property:  
$$Y = A ⊙ (K + C) = \frac{A}{1 + A \cdot (K + C)}$$
Then:  
$$Y ⊘ \frac{1}{A} = \frac{Y}{1 - \frac{1}{A} \cdot Y} = \frac{\frac{A}{1 + A \cdot (K + C)}}{1 - \frac{1}{1 + A \cdot (K + C)}} = \frac{1}{K + C}$$  
Thus:
$\left( Y ⊘ \frac{1}{A} \right)^{-1} = K + C \quad \square$

## 10.4 Subtraction Through KMR Operators

### 10.4.1 General Case Expression
For any $A ≠ 0$, the difference of two parameters $K$ and $C$ can be expressed as:  
$$K - C = - \left( \left( (A ⊘ K) ⊙ C \right) ⊘ \frac{1}{A} \right)^{-1} = \left( \left( (-A ⊘ K) ⊙ C \right) ⊘ \frac{1}{A} \right)^{-1}$$

### 10.4.2 Special Case (A = 1)  
When $A = 1$, the expression simplifies to:  
$$K - C = - \left( \left( (1 ⊘ K) ⊙ C \right) ⊘ 1 \right)^{-1} = \left( \left( (-1 ⊘ K) ⊙ C \right) ⊘ 1 \right)^{-1}$$

### 10.4.3 Proof
Using the scaling property and the revised parameter extraction:  
$$[K - C = - \left( \left( (A ⊘ K) ⊙ C \right) ⊘ \frac{1}{A} \right)^{-1} = \left( -1 \cdot \left( \left( (A ⊘ K) ⊙ C \right) ⊘ \frac{1}{A} \right) \right)^{-1} = \left( \left( (-A ⊘ K) ⊙ C \right) ⊘ \frac{1}{A} \right)^{-1} \quad \square]$$

## 10.5 Numerical Examples

### 10.5.1 Addition Example
Let $A = 2$, $K = 3$, $C = 4$:
- $2 ⊙ 3 = \frac{2}{1 + 2 \cdot 3} = \frac{2}{7} ≈ 0.2857$
- $(2 ⊙ 3) ⊙ 4 = \frac{2/7}{1 + (2/7) \cdot 4} = \frac{2}{15} ≈ 0.1333$
- $\left( (2 ⊙ 3) ⊙ 4 \right) ⊘ \frac{1}{2} = \frac{2/15}{1 - (1/2) \cdot (2/15)} = \frac{2/15}{14/15} = \frac{1}{7}$
- $\left( \frac{1}{7} \right)^{-1} = 7 = 3 + 4$

### 10.5.2 Subtraction Example
Let $A = 1$, $K = 5$, $C = 2$:
- $1 ⊘ 5 = \frac{1}{1 - 1 \cdot 5} = -\frac{1}{4} = -0.25$
- $(1 ⊘ 5) ⊙ 2 = \frac{-0.25}{1 + (-0.25) \cdot 2} = \frac{-0.25}{0.5} = -0.5$
- $(-0.5) ⊘ 1 = \frac{-0.5}{1 - 1 \cdot (-0.5)} = \frac{-0.5}{1.5} = -\frac{1}{3}$
- $-\left( -\frac{1}{3} \right)^{-1} = -(-3) = 3 = 5 - 2$

**Alternative using the symmetric form**:
- $(-1) ⊘ 5 = \frac{-1}{1 - 5 \cdot (-1)} = \frac{-1}{6} ≈ -0.1667$
- $(-1 ⊘ 5) ⊙ 2 = \frac{-0.1667}{1 + 2 \cdot (-0.1667)} = \frac{-0.1667}{0.6667} = -0.25$
- $(-0.25) ⊘ 1 = \frac{-0.25}{1 - 1 \cdot (-0.25)} = \frac{-0.25}{1.25} = -0.2$
- $(-0.2)^{-1} = -5$ (demonstrating the symmetric form)

## 10.6 Python Implementation

```python
def kmr_add(A: float, K: float, C: float) -> float:
    """Compute K + C using KMR operators."""
    if abs(A) < 1e-15:  # Handle A ≈ 0 case
        return K + C
    X = kmr_direct(A, K)
    Y = kmr_direct(X, C)
    Z = kmr_inverse(Y, 1/A)
    return 1/Z

def kmr_sub(A: float, K: float, C: float) -> float:
    """Compute K - C using KMR operators."""
    if abs(A) < 1e-15:  # Handle A ≈ 0 case
        return K - C
    # Using the standard form
    X = kmr_inverse(A, K)
    Y = kmr_direct(X, C)
    Z = kmr_inverse(Y, 1/A)
    return -1/Z
    
    # Alternative using symmetric form
    # X = kmr_inverse(-A, K)
    # Y = kmr_direct(X, C)
    # Z = kmr_inverse(Y, 1/A)
    # return 1/Z
```


	
##  10.7 Implications and Future Directions
These results demonstrate that:

Basic arithmetic operations emerge naturally from KMR operator composition

Linear arithmetic represents a special case of nonlinear KMR transformations

The scaling property provides additional mathematical elegance to the framework

The symmetric forms reveal deeper algebraic structure of KMR operations

The framework provides a unified approach to linear and nonlinear mathematics

Future research directions include:

Extension to multiplication and division through KMR operators

Applications in nonlinear system modeling and control theory

Connections to fractional calculus and non-integer operations

Implementation in computational mathematics and symbolic computation systems

##  10.8 Conclusion
The expression of arithmetic operations through KMR operators provides further evidence for the fundamental nature of nonlinear transformations in mathematics. This approach offers a unified framework where linear arithmetic emerges as a special case of more general nonlinear operations, potentially leading to new insights in both theoretical and applied mathematics.


<!-- License: CC BY-SA 4.0 (see LICENSE-CC.md) -->
